Proved Init_simp

probability/probabilistic_relations/Examples/machine_learning_examples/utp_prob_rel_cancer_diagnosis.thy
@@ -54,13 +54,16 @@ definition Init :: "state prhfun" where
   TestRel
 "
 
-lemma TestRel_simp: 
-  "TestRel = prfun_of_rvfun (
+definition TestRel_altdef :: "state rvhfun" where
+"TestRel_altdef = (
     (\<lbrakk>lt\<^sup>> = Pos\<rbrakk>\<^sub>\<I>\<^sub>e * \<lbrakk>c\<^sup><\<rbrakk>\<^sub>\<I>\<^sub>e * \<lbrakk>c\<^sup>> = c\<^sup><\<rbrakk>\<^sub>\<I>\<^sub>e * p\<^sub>2) + 
     (\<lbrakk>lt\<^sup>> = Neg\<rbrakk>\<^sub>\<I>\<^sub>e * \<lbrakk>c\<^sup><\<rbrakk>\<^sub>\<I>\<^sub>e * \<lbrakk>c\<^sup>> = c\<^sup><\<rbrakk>\<^sub>\<I>\<^sub>e *(1-p\<^sub>2)) + 
     (\<lbrakk>lt\<^sup>> = Pos\<rbrakk>\<^sub>\<I>\<^sub>e * \<lbrakk>\<not>c\<^sup><\<rbrakk>\<^sub>\<I>\<^sub>e * \<lbrakk>c\<^sup>> = c\<^sup><\<rbrakk>\<^sub>\<I>\<^sub>e *p\<^sub>3) + 
     (\<lbrakk>lt\<^sup>> = Neg\<rbrakk>\<^sub>\<I>\<^sub>e * \<lbrakk>\<not>c\<^sup><\<rbrakk>\<^sub>\<I>\<^sub>e * \<lbrakk>c\<^sup>> = c\<^sup><\<rbrakk>\<^sub>\<I>\<^sub>e *(1-p\<^sub>3)))\<^sub>e"
-  apply (simp only: TestRel_def)
+
+lemma TestRel_simp: 
+  "TestRel = prfun_of_rvfun TestRel_altdef"
+  apply (simp only: TestRel_def TestRel_altdef_def)
   apply (simp add: prfun_seqcomp_right_unit)
   apply (simp add: prfun_pcond_altdef)
   apply (simp only: pchoice_def passigns_def)
@@ -79,18 +82,241 @@ lemma TestRel_simp:
   apply (subst fun_eq_iff)
   by (pred_simp)
 
-lemma 
+lemma TestRel_altdef_final: "is_final_distribution TestRel_altdef"
+  apply (simp add: dist_defs expr_defs TestRel_altdef_def)
+  apply (pred_auto)
+proof -
+  fix c
+  have pos_false: "{s::state. lt\<^sub>v s = Pos \<and> \<not> c\<^sub>v s} = {\<lparr>c\<^sub>v = False,lt\<^sub>v = Pos\<rparr>}"
+    apply (simp add: set_eq_iff)
+    apply (rule allI)
+    apply (rule iffI)
+    by simp+
+  have neg_false: "{s::state. lt\<^sub>v s = Neg \<and> \<not> c\<^sub>v s} = {\<lparr>c\<^sub>v = False,lt\<^sub>v = Neg\<rparr>}"
+    apply (simp add: set_eq_iff)
+    apply (rule allI)
+    apply (rule iffI)
+    by simp+
+  have summable_pos_false: "(\<lambda>x::state. if lt\<^sub>v x = Pos \<and> \<not> c\<^sub>v x then 1::\<real> else (0::\<real>)) summable_on UNIV"
+    apply (rule infsum_constant_finite_states_summable)
+    by (simp add: pos_false)
+  have summable_neg_false: "(\<lambda>x::state. if lt\<^sub>v x = Neg \<and> \<not> c\<^sub>v x then 1::\<real> else (0::\<real>)) summable_on UNIV"
+    apply (rule infsum_constant_finite_states_summable)
+    by (simp add: neg_false)
+  have "(\<Sum>\<^sub>\<infinity>s::state.
+          (if lt\<^sub>v s = Pos then 1::\<real> else (0::\<real>)) * (if \<not> c\<^sub>v s then 1::\<real> else (0::\<real>)) / (20::\<real>) +
+          (if lt\<^sub>v s = Neg then 1::\<real> else (0::\<real>)) * (if \<not> c\<^sub>v s then 1::\<real> else (0::\<real>)) * (19::\<real>) / (20::\<real>)) =
+       (\<Sum>\<^sub>\<infinity>s::state.
+          (if lt\<^sub>v s = Pos \<and> \<not> c\<^sub>v s then 1::\<real> else (0::\<real>)) / (20::\<real>) +
+          (if lt\<^sub>v s = Neg \<and> \<not> c\<^sub>v s then 1::\<real> else (0::\<real>)) * (19::\<real>) / (20::\<real>))"
+    by (smt (verit, ccfv_SIG) infsum_cong mult_cancel_right1 mult_eq_0_iff)
+  also have "... = (\<Sum>\<^sub>\<infinity>s::state. (if lt\<^sub>v s = Pos \<and> \<not> c\<^sub>v s then 1::\<real> else (0::\<real>)) / (20::\<real>)) +
+          (\<Sum>\<^sub>\<infinity>s::state. (if lt\<^sub>v s = Neg \<and> \<not> c\<^sub>v s then 1::\<real> else (0::\<real>)) * (19::\<real>) / (20::\<real>))"
+    apply (subst infsum_add)
+    apply (rule summable_on_cdiv_left)
+    using summable_pos_false apply blast
+    apply (rule summable_on_cdiv_left)
+    apply (rule summable_on_cmult_left)
+    using summable_neg_false apply blast
+    by simp
+  also have "... = 1"
+    apply (subst infsum_cdiv_left)
+    using summable_pos_false apply blast
+    apply (subst infsum_cdiv_left)
+    apply (rule summable_on_cmult_left)
+    using summable_neg_false apply blast
+    apply (subst infsum_constant_finite_states)
+     apply (simp add: pos_false)
+    apply (subst infsum_cmult_left)
+    using summable_neg_false apply blast
+    apply (subst infsum_constant_finite_states)
+    apply (simp add: neg_false)
+    by (simp add: pos_false neg_false)
+  then show "(\<Sum>\<^sub>\<infinity>s::state.
+          (if lt\<^sub>v s = Pos then 1::\<real> else (0::\<real>)) * (if \<not> c\<^sub>v s then 1::\<real> else (0::\<real>)) / (20::\<real>) +
+          (if lt\<^sub>v s = Neg then 1::\<real> else (0::\<real>)) * (if \<not> c\<^sub>v s then 1::\<real> else (0::\<real>)) * (19::\<real>) / (20::\<real>)) =
+       (1::\<real>)"
+    using calculation by presburger
+next
+  fix c
+  have pos_true: "{s::state. lt\<^sub>v s = Pos \<and> c\<^sub>v s} = {\<lparr>c\<^sub>v = True,lt\<^sub>v = Pos\<rparr>}"
+    apply (simp add: set_eq_iff)
+    apply (rule allI)
+    apply (rule iffI)
+    by simp+
+  have neg_true: "{s::state. lt\<^sub>v s = Neg \<and> c\<^sub>v s} = {\<lparr>c\<^sub>v = True,lt\<^sub>v = Neg\<rparr>}"
+    apply (simp add: set_eq_iff)
+    apply (rule allI)
+    apply (rule iffI)
+    by simp+
+  have summable_pos_true: "(\<lambda>x::state. if lt\<^sub>v x = Pos \<and> c\<^sub>v x then 1::\<real> else (0::\<real>)) summable_on UNIV"
+    apply (rule infsum_constant_finite_states_summable)
+    by (simp add: pos_true)
+  have summable_neg_true: "(\<lambda>x::state. if lt\<^sub>v x = Neg \<and> c\<^sub>v x then 1::\<real> else (0::\<real>)) summable_on UNIV"
+    apply (rule infsum_constant_finite_states_summable)
+    by (simp add: neg_true)
+  have "(\<Sum>\<^sub>\<infinity>s::state.
+          (if lt\<^sub>v s = Pos then 1::\<real> else (0::\<real>)) * (if c\<^sub>v s then 1::\<real> else (0::\<real>)) * (89::\<real>) / (100::\<real>) +
+          (if lt\<^sub>v s = Neg then 1::\<real> else (0::\<real>)) * (if c\<^sub>v s then 1::\<real> else (0::\<real>)) * (11::\<real>) / (100::\<real>)) =
+       (\<Sum>\<^sub>\<infinity>s::state.
+          (if lt\<^sub>v s = Pos \<and> c\<^sub>v s then 1::\<real> else (0::\<real>))* (89::\<real>) / (100::\<real>) +
+          (if lt\<^sub>v s = Neg \<and> c\<^sub>v s then 1::\<real> else (0::\<real>)) * (11::\<real>) / (100::\<real>))"
+    by (smt (verit, ccfv_SIG) infsum_cong mult_cancel_right1 mult_eq_0_iff)
+  also have "... = (\<Sum>\<^sub>\<infinity>s::state. (if lt\<^sub>v s = Pos \<and> c\<^sub>v s then 1::\<real> else (0::\<real>)) * (89::\<real>) / (100::\<real>)) +
+          (\<Sum>\<^sub>\<infinity>s::state. (if lt\<^sub>v s = Neg \<and> c\<^sub>v s then 1::\<real> else (0::\<real>)) * (11::\<real>) / (100::\<real>))"
+    apply (subst infsum_add)
+    apply (rule summable_on_cdiv_left)
+    apply (rule summable_on_cmult_left)
+    using summable_pos_true apply blast
+    apply (rule summable_on_cdiv_left)
+    apply (rule summable_on_cmult_left)
+    using summable_neg_true apply blast
+    by simp
+  also have "... = 1"
+    apply (subst infsum_cdiv_left)
+    apply (rule summable_on_cmult_left)
+    using summable_pos_true apply blast
+    apply (subst infsum_cdiv_left)
+     apply (rule summable_on_cmult_left)
+    using summable_neg_true apply blast
+    apply (subst infsum_cmult_left)
+    using summable_pos_true apply blast
+    apply (subst infsum_constant_finite_states)
+     apply (simp add: pos_true)
+    apply (subst infsum_cmult_left)
+    using summable_neg_true apply blast
+    apply (subst infsum_constant_finite_states)
+    apply (simp add: neg_true)
+    by (simp add: pos_true neg_true)
+
+  then show "(\<Sum>\<^sub>\<infinity>s::state.
+          (if lt\<^sub>v s = Pos then 1::\<real> else (0::\<real>)) * (if c\<^sub>v s then 1::\<real> else (0::\<real>)) * (89::\<real>) / (100::\<real>) +
+          (if lt\<^sub>v s = Neg then 1::\<real> else (0::\<real>)) * (if c\<^sub>v s then 1::\<real> else (0::\<real>)) * (11::\<real>) / (100::\<real>)) =
+       (1::\<real>)"
+    using calculation by presburger
+qed
+
+lemma Init_simp:
   shows "Init = prfun_of_rvfun (
-    (\<lbrakk>lt\<^sup>> = Pos\<rbrakk>\<^sub>\<I>\<^sub>e * \<lbrakk>c\<^sup><\<rbrakk>\<^sub>\<I>\<^sub>e * \<lbrakk>c\<^sup>> = c\<^sup><\<rbrakk>\<^sub>\<I>\<^sub>e * p\<^sub>1 * p\<^sub>2) + 
-    (\<lbrakk>lt\<^sup>> = Neg\<rbrakk>\<^sub>\<I>\<^sub>e * \<lbrakk>c\<^sup><\<rbrakk>\<^sub>\<I>\<^sub>e * \<lbrakk>c\<^sup>> = c\<^sup><\<rbrakk>\<^sub>\<I>\<^sub>e * p\<^sub>1 * (1-p\<^sub>2)) + 
-    (\<lbrakk>lt\<^sup>> = Pos\<rbrakk>\<^sub>\<I>\<^sub>e * \<lbrakk>\<not>c\<^sup><\<rbrakk>\<^sub>\<I>\<^sub>e * \<lbrakk>c\<^sup>> = c\<^sup><\<rbrakk>\<^sub>\<I>\<^sub>e * (1-p\<^sub>1) * p\<^sub>2) + 
-    (\<lbrakk>lt\<^sup>> = Neg\<rbrakk>\<^sub>\<I>\<^sub>e * \<lbrakk>\<not>c\<^sup><\<rbrakk>\<^sub>\<I>\<^sub>e * \<lbrakk>c\<^sup>> = c\<^sup><\<rbrakk>\<^sub>\<I>\<^sub>e * (1-p\<^sub>1) * (1-p\<^sub>2))
+    (\<lbrakk>lt\<^sup>> = Pos\<rbrakk>\<^sub>\<I>\<^sub>e * \<lbrakk>c\<^sup>>\<rbrakk>\<^sub>\<I>\<^sub>e * p\<^sub>1 * p\<^sub>2) + 
+    (\<lbrakk>lt\<^sup>> = Neg\<rbrakk>\<^sub>\<I>\<^sub>e * \<lbrakk>c\<^sup>>\<rbrakk>\<^sub>\<I>\<^sub>e * p\<^sub>1 * (1-p\<^sub>2)) + 
+    (\<lbrakk>lt\<^sup>> = Pos\<rbrakk>\<^sub>\<I>\<^sub>e * \<lbrakk>\<not>c\<^sup>>\<rbrakk>\<^sub>\<I>\<^sub>e * (1-p\<^sub>1) * p\<^sub>3) + 
+    (\<lbrakk>lt\<^sup>> = Neg\<rbrakk>\<^sub>\<I>\<^sub>e * \<lbrakk>\<not>c\<^sup>>\<rbrakk>\<^sub>\<I>\<^sub>e * (1-p\<^sub>1) * (1-p\<^sub>3))
 )\<^sub>e"
-  (* apply (simp only: Init_def)
+  apply (simp only: Init_def)
   apply (simp add: TestRel_simp)
   apply (simp only: pseqcomp_def)
-  *)
+  apply (subst rvfun_inverse) 
+  using TestRel_altdef_final rvfun_prob_sum1_summable'(1) apply blast
+  apply (subst prfun_pchoice_assigns_inverse_c')
+  apply (simp add: TestRel_altdef_def)
+  apply (expr_simp_1)
+  apply (simp add: real2eureal_inverse)
+  apply (rule HOL.arg_cong[where f="prfun_of_rvfun"])
+  apply (subst fun_eq_iff)
+  apply (pred_auto)
+proof -
+  fix lt c
+  let ?f = "(\<Sum>\<^sub>\<infinity>v\<^sub>0::state.
+          ((if v\<^sub>0 = \<lparr>c\<^sub>v = True, lt\<^sub>v = lt\<rparr> then 1::\<real> else (0::\<real>)) / (500::\<real>) +
+           (499::\<real>) * (if v\<^sub>0 = \<lparr>c\<^sub>v = False, lt\<^sub>v = lt\<rparr> then 1::\<real> else (0::\<real>)) / (500::\<real>)) *
+          ((if c\<^sub>v v\<^sub>0 then 1::\<real> else (0::\<real>)) * (if \<not> c\<^sub>v v\<^sub>0 then 1::\<real> else (0::\<real>)) * (89::\<real>) / (100::\<real>) +
+           (if \<not> c\<^sub>v v\<^sub>0 then 1::\<real> else (0::\<real>)) * (if \<not> c\<^sub>v v\<^sub>0 then 1::\<real> else (0::\<real>)) / (20::\<real>)))"
+  have "?f = (\<Sum>\<^sub>\<infinity>v\<^sub>0::state.
+          ((if v\<^sub>0 = \<lparr>c\<^sub>v = True, lt\<^sub>v = lt\<rparr> then 1::\<real> else (0::\<real>)) / (500::\<real>) +
+           (499::\<real>) * (if v\<^sub>0 = \<lparr>c\<^sub>v = False, lt\<^sub>v = lt\<rparr> then 1::\<real> else (0::\<real>)) / (500::\<real>)) *
+          ((if \<not> c\<^sub>v v\<^sub>0 then 1::\<real> else (0::\<real>)) * (if \<not> c\<^sub>v v\<^sub>0 then 1::\<real> else (0::\<real>)) / (20::\<real>)))"
+    by (smt (verit) divide_eq_0_iff infsum_cong mult_eq_0_iff)
+  also have "... = (\<Sum>\<^sub>\<infinity>v\<^sub>0::state.
+          ((499::\<real>) * (if v\<^sub>0 = \<lparr>c\<^sub>v = False, lt\<^sub>v = lt\<rparr> then 1::\<real> else (0::\<real>)) / (500::\<real>)) *
+          ((if \<not> c\<^sub>v v\<^sub>0 then 1::\<real> else (0::\<real>)) / (20::\<real>)))"
+    by (simp add: infsum_cong)
+  also have "... = (\<Sum>\<^sub>\<infinity>v\<^sub>0 \<in> {\<lparr>c\<^sub>v = False, lt\<^sub>v = lt\<rparr>}. ((499::\<real>) / (10000::\<real>)))"
+    apply (subst infsum_cong_neutral[where S="UNIV" and T="{\<lparr>c\<^sub>v = False, lt\<^sub>v = lt\<rparr>}" and 
+         f = "\<lambda>v\<^sub>0. ((499::\<real>) * (if v\<^sub>0 = \<lparr>c\<^sub>v = False, lt\<^sub>v = lt\<rparr> then 1::\<real> else (0::\<real>)) / (500::\<real>)) *
+          ((if \<not> c\<^sub>v v\<^sub>0 then 1::\<real> else (0::\<real>)) / (20::\<real>))" and
+         g = "\<lambda>v\<^sub>0. ((499::\<real>) / (10000::\<real>))"])
+    apply blast
+    by simp+
+  also have "... = ((499::\<real>) / (10000::\<real>))"
+    by simp
+  then show "(\<Sum>\<^sub>\<infinity>v\<^sub>0::state.
+          ((if v\<^sub>0 = \<lparr>c\<^sub>v = True, lt\<^sub>v = lt\<rparr> then 1::\<real> else (0::\<real>)) / (500::\<real>) +
+           (499::\<real>) * (if v\<^sub>0 = \<lparr>c\<^sub>v = False, lt\<^sub>v = lt\<rparr> then 1::\<real> else (0::\<real>)) / (500::\<real>)) *
+          ((if c\<^sub>v v\<^sub>0 then 1::\<real> else (0::\<real>)) * (if \<not> c\<^sub>v v\<^sub>0 then 1::\<real> else (0::\<real>)) * (89::\<real>) / (100::\<real>) +
+           (if \<not> c\<^sub>v v\<^sub>0 then 1::\<real> else (0::\<real>)) * (if \<not> c\<^sub>v v\<^sub>0 then 1::\<real> else (0::\<real>)) / (20::\<real>))) *
+       (10000::\<real>) = (499::\<real>)"
+    using calculation by linarith
+next
+  fix lt c
+  have "(\<Sum>\<^sub>\<infinity>v\<^sub>0::state.
+          ((if v\<^sub>0 = \<lparr>c\<^sub>v = True, lt\<^sub>v = lt\<rparr> then 1::\<real> else (0::\<real>)) / (500::\<real>) +
+           (499::\<real>) * (if v\<^sub>0 = \<lparr>c\<^sub>v = False, lt\<^sub>v = lt\<rparr> then 1::\<real> else (0::\<real>)) / (500::\<real>)) *
+          ((if c\<^sub>v v\<^sub>0 then 1::\<real> else (0::\<real>)) * (if c\<^sub>v v\<^sub>0 then 1::\<real> else (0::\<real>)) * (89::\<real>) / (100::\<real>) +
+           (if \<not> c\<^sub>v v\<^sub>0 then 1::\<real> else (0::\<real>)) * (if c\<^sub>v v\<^sub>0 then 1::\<real> else (0::\<real>)) / (20::\<real>)))
+    = (\<Sum>\<^sub>\<infinity>v\<^sub>0::state. ((if v\<^sub>0 = \<lparr>c\<^sub>v = True, lt\<^sub>v = lt\<rparr> then 1::\<real> else (0::\<real>)) * (89::\<real>) / (50000::\<real>)))"
+    apply (subst infsum_cong[where g = "\<lambda>v\<^sub>0::state. ((if v\<^sub>0 = \<lparr>c\<^sub>v = True, lt\<^sub>v = lt\<rparr> then 1::\<real> else (0::\<real>)) * (89::\<real>) / (50000::\<real>))"])
+    by auto
+  also have "... = (\<Sum>\<^sub>\<infinity>v\<^sub>0::state\<in>{\<lparr>c\<^sub>v = True, lt\<^sub>v = lt\<rparr>}. ((89::\<real>) / (50000::\<real>)))"
+    apply (subst infsum_cong_neutral[where S="UNIV" and T="{\<lparr>c\<^sub>v = True, lt\<^sub>v = lt\<rparr>}" and 
+         f = "\<lambda>v\<^sub>0. (if v\<^sub>0 = \<lparr>c\<^sub>v = True, lt\<^sub>v = lt\<rparr> then 1::\<real> else (0::\<real>)) * (89::\<real>) / (50000::\<real>)" and
+         g = "\<lambda>v\<^sub>0. ((89::\<real>) / (50000::\<real>))"])
+    by simp+
+  then show "(\<Sum>\<^sub>\<infinity>v\<^sub>0::state.
+          ((if v\<^sub>0 = \<lparr>c\<^sub>v = True, lt\<^sub>v = lt\<rparr> then 1::\<real> else (0::\<real>)) / (500::\<real>) +
+           (499::\<real>) * (if v\<^sub>0 = \<lparr>c\<^sub>v = False, lt\<^sub>v = lt\<rparr> then 1::\<real> else (0::\<real>)) / (500::\<real>)) *
+          ((if c\<^sub>v v\<^sub>0 then 1::\<real> else (0::\<real>)) * (if c\<^sub>v v\<^sub>0 then 1::\<real> else (0::\<real>)) * (89::\<real>) / (100::\<real>) +
+           (if \<not> c\<^sub>v v\<^sub>0 then 1::\<real> else (0::\<real>)) * (if c\<^sub>v v\<^sub>0 then 1::\<real> else (0::\<real>)) / (20::\<real>))) *
+       (50000::\<real>) = (89::\<real>)"
+    using calculation by fastforce
+next
+  fix lt c
+  have "(\<Sum>\<^sub>\<infinity>v\<^sub>0::state.
+          ((if v\<^sub>0 = \<lparr>c\<^sub>v = True, lt\<^sub>v = lt\<rparr> then 1::\<real> else (0::\<real>)) / (500::\<real>) +
+           (499::\<real>) * (if v\<^sub>0 = \<lparr>c\<^sub>v = False, lt\<^sub>v = lt\<rparr> then 1::\<real> else (0::\<real>)) / (500::\<real>)) *
+          ((if c\<^sub>v v\<^sub>0 then 1::\<real> else (0::\<real>)) * (if \<not> c\<^sub>v v\<^sub>0 then 1::\<real> else (0::\<real>)) * (11::\<real>) / (100::\<real>) +
+           (if \<not> c\<^sub>v v\<^sub>0 then 1::\<real> else (0::\<real>)) * (if \<not> c\<^sub>v v\<^sub>0 then 1::\<real> else (0::\<real>)) * (19::\<real>) / (20::\<real>))) =
+      (\<Sum>\<^sub>\<infinity>v\<^sub>0::state.
+          ((9481::\<real>) * (if v\<^sub>0 = \<lparr>c\<^sub>v = False, lt\<^sub>v = lt\<rparr> then 1::\<real> else (0::\<real>)) / (10000::\<real>)))"
+    apply (subst infsum_cong[where g = "\<lambda>v\<^sub>0::state. ((9481::\<real>) * (if v\<^sub>0 = \<lparr>c\<^sub>v = False, lt\<^sub>v = lt\<rparr> then 1::\<real> else (0::\<real>)) / (10000::\<real>))"])
+    by auto
+  also have "... = (\<Sum>\<^sub>\<infinity>v\<^sub>0::state\<in>{\<lparr>c\<^sub>v = False, lt\<^sub>v = lt\<rparr>}. ((9481::\<real>) / (10000::\<real>)))"
+    apply (subst infsum_cong_neutral[where S="UNIV" and T="{\<lparr>c\<^sub>v = False, lt\<^sub>v = lt\<rparr>}" and 
+         f = "\<lambda>v\<^sub>0. ((9481::\<real>) * (if v\<^sub>0 = \<lparr>c\<^sub>v = False, lt\<^sub>v = lt\<rparr> then 1::\<real> else (0::\<real>)) / (10000::\<real>))" and
+         g = "\<lambda>v\<^sub>0. ((9481::\<real>) / (10000::\<real>))"])
+    by simp+
+  then show "(\<Sum>\<^sub>\<infinity>v\<^sub>0::state.
+        ((if v\<^sub>0 = \<lparr>c\<^sub>v = True, lt\<^sub>v = lt\<rparr> then 1::\<real> else (0::\<real>)) / (500::\<real>) +
+         (499::\<real>) * (if v\<^sub>0 = \<lparr>c\<^sub>v = False, lt\<^sub>v = lt\<rparr> then 1::\<real> else (0::\<real>)) / (500::\<real>)) *
+        ((if c\<^sub>v v\<^sub>0 then 1::\<real> else (0::\<real>)) * (if \<not> c\<^sub>v v\<^sub>0 then 1::\<real> else (0::\<real>)) * (11::\<real>) / (100::\<real>) +
+         (if \<not> c\<^sub>v v\<^sub>0 then 1::\<real> else (0::\<real>)) * (if \<not> c\<^sub>v v\<^sub>0 then 1::\<real> else (0::\<real>)) * (19::\<real>) / (20::\<real>))) *
+     (10000::\<real>) = (9481::\<real>)"
+    using calculation by fastforce
+next
+  fix lt c
+  have "(\<Sum>\<^sub>\<infinity>v\<^sub>0::state.
+          ((if v\<^sub>0 = \<lparr>c\<^sub>v = True, lt\<^sub>v = lt\<rparr> then 1::\<real> else (0::\<real>)) / (500::\<real>) +
+           (499::\<real>) * (if v\<^sub>0 = \<lparr>c\<^sub>v = False, lt\<^sub>v = lt\<rparr> then 1::\<real> else (0::\<real>)) / (500::\<real>)) *
+          ((if c\<^sub>v v\<^sub>0 then 1::\<real> else (0::\<real>)) * (if c\<^sub>v v\<^sub>0 then 1::\<real> else (0::\<real>)) * (11::\<real>) / (100::\<real>) +
+           (if \<not> c\<^sub>v v\<^sub>0 then 1::\<real> else (0::\<real>)) * (if c\<^sub>v v\<^sub>0 then 1::\<real> else (0::\<real>)) * (19::\<real>) / (20::\<real>)))
+      = (\<Sum>\<^sub>\<infinity>v\<^sub>0::state. (if v\<^sub>0 = \<lparr>c\<^sub>v = True, lt\<^sub>v = lt\<rparr> then 1::\<real> else (0::\<real>)) *(11::\<real>) / (50000::\<real>))"
+    apply (subst infsum_cong[where g = "\<lambda>v\<^sub>0::state. (if v\<^sub>0 = \<lparr>c\<^sub>v = True, lt\<^sub>v = lt\<rparr> then 1::\<real> else (0::\<real>)) *(11::\<real>) / (50000::\<real>)"])
+    by auto
+  also have "... = (\<Sum>\<^sub>\<infinity>v\<^sub>0::state\<in>{\<lparr>c\<^sub>v = True, lt\<^sub>v = lt\<rparr>}. ((11::\<real>) / (50000::\<real>)))"
+    apply (subst infsum_cong_neutral[where S="UNIV" and T="{\<lparr>c\<^sub>v = True, lt\<^sub>v = lt\<rparr>}" and 
+         f = "\<lambda>v\<^sub>0. (if v\<^sub>0 = \<lparr>c\<^sub>v = True, lt\<^sub>v = lt\<rparr> then 1::\<real> else (0::\<real>)) *(11::\<real>) / (50000::\<real>)" and
+         g = "\<lambda>v\<^sub>0. ((11::\<real>) / (50000::\<real>))"])
+    by simp+
+  then show "(\<Sum>\<^sub>\<infinity>v\<^sub>0::state.
+          ((if v\<^sub>0 = \<lparr>c\<^sub>v = True, lt\<^sub>v = lt\<rparr> then 1::\<real> else (0::\<real>)) / (500::\<real>) +
+           (499::\<real>) * (if v\<^sub>0 = \<lparr>c\<^sub>v = False, lt\<^sub>v = lt\<rparr> then 1::\<real> else (0::\<real>)) / (500::\<real>)) *
+          ((if c\<^sub>v v\<^sub>0 then 1::\<real> else (0::\<real>)) * (if c\<^sub>v v\<^sub>0 then 1::\<real> else (0::\<real>)) * (11::\<real>) / (100::\<real>) +
+           (if \<not> c\<^sub>v v\<^sub>0 then 1::\<real> else (0::\<real>)) * (if c\<^sub>v v\<^sub>0 then 1::\<real> else (0::\<real>)) * (19::\<real>) / (20::\<real>))) *
+       (50000::\<real>) = (11::\<real>)"
+    using calculation by force
+qed
 
+(*
   apply (simp only: Init_def TestRel_def)
   apply (simp only: pcond_def)
   apply (simp only: pseqcomp_def)
@@ -138,5 +364,5 @@ lemma
   apply simp+
 
   apply (simp add: pfun_defs)
-
+*)
 end
